refactor: use usual Lean naming conventions

Lustrean/Domain/Domain.lean
@@ -26,147 +26,147 @@ infixr:60 " ⊔ " => join
 infixr:70 " ⊓ " => meet
 
 namespace BoundedLattice
-  variable {α : Type} [ι : BoundedLattice α]
+variable {α : Type} [ι : BoundedLattice α]
 
-  attribute [simp] bot top join meet
-  attribute [simp]
-  join_associative join_absorption join_bot join_top
-  meet_associative meet_absorption meet_bot meet_top
+attribute [simp] bot top join meet
+attribute [simp]
+join_associative join_absorption join_bot join_top
+meet_associative meet_absorption meet_bot meet_top
 
-  def is_bot : α → Prop :=
-    (· = ⊥)
+def IsBot : α → Prop :=
+  (· = ⊥)
 
-  def is_subset : α → α → Prop :=
-    fun x y => x = meet x y
+def IsSubset : α → α → Prop :=
+  fun x y => x = meet x y
 
-  infixr:50 " ⊑ " => is_subset
+infixr:50 " ⊑ " => IsSubset
 
-  theorem trans : ∀ {x y z : α}, x ⊑ y → y ⊑ z → x ⊑ z := by
-    intros x y z Hx Hy
-    unfold is_subset at *
-    rw [Hx]
-    conv =>
-      lhs
-      rw [Hy]
-    rw [meet_associative]
+theorem trans : ∀ {x y z : α}, x ⊑ y → y ⊑ z → x ⊑ z := by
+  intros x y z Hx Hy
+  unfold IsSubset at *
+  rw [Hx]
+  conv =>
+    lhs
+    rw [Hy]
+  rw [meet_associative]
 
-  instance {α : Type} [ι : BoundedLattice α] : Trans (@is_subset α ι) (@is_subset α ι) (@is_subset α ι) where
-    trans := trans
+instance {α : Type} [ι : BoundedLattice α] : Trans (@IsSubset α ι) (@IsSubset α ι) (@IsSubset α ι) where
+  trans := trans
 
-  theorem bot_min : ∀ {x : α}, ⊥ ⊑ x := by
-    intros x
-    unfold is_subset
-    simp [meet_commutative]
+theorem bot_min : ∀ {x : α}, ⊥ ⊑ x := by
+  intros x
+  unfold IsSubset
+  simp [meet_commutative]
 
-  theorem antisymm : ∀ {x y : α}, x ⊑ y → y ⊑ x → x = y := by
-    intros x y H H'
-    unfold is_subset at *
-    rw [meet_commutative] at H'
-    rw [H]
-    symm
-    assumption
+theorem antisymm : ∀ {x y : α}, x ⊑ y → y ⊑ x → x = y := by
+  intros x y H H'
+  unfold IsSubset at *
+  rw [meet_commutative] at H'
+  rw [H]
+  symm
+  assumption
 
-  instance {α : Type} [ι : BoundedLattice α] : Std.Antisymm (@is_subset α ι) where
-    antisymm := @antisymm _ _
+instance {α : Type} [ι : BoundedLattice α] : Std.Antisymm (@IsSubset α ι) where
+  antisymm := @antisymm _ _
 
-  @[simp]
-  theorem min_bot_is_bot : ∀ {x : α}, x ⊑ ⊥ → x = bot := by
-    intros x H
-    apply antisymm <;> [
-      assumption ;
-      apply bot_min
-    ]
+@[simp]
+theorem min_bot_is_bot : ∀ {x : α}, x ⊑ ⊥ → x = bot := by
+  intros x H
+  apply antisymm <;> [
+    assumption ;
+    apply bot_min
+  ]
 
-  theorem min_join_left : ∀ {x y : α}, x ⊑ x ⊔ y := by
-    intros x y
-    unfold is_subset
-    symm
-    apply meet_absorption
+theorem min_join_left : ∀ {x y : α}, x ⊑ x ⊔ y := by
+  intros x y
+  unfold IsSubset
+  symm
+  apply meet_absorption
 
-  theorem min_join_right : ∀ {x y : α}, y ⊑ x ⊔ y := by
-    intros
-    rw [join_commutative]
-    apply min_join_left
+theorem min_join_right : ∀ {x y : α}, y ⊑ x ⊔ y := by
+  intros
+  rw [join_commutative]
+  apply min_join_left
 
-  theorem join_eq_bot_iff_bot : ∀ {x y : α}, x ⊔ y = ⊥ ↔ x = ⊥ ∧ y = ⊥ := by
-    intros x y
-    constructor
-    · intros H
-      have : ∀ (a b : α), a ⊔ b = ⊥ → a = ⊥ := by
-        intros a b Ha
-        have : a = a ⊓ (a ⊔ b) := by simp
-        rw [this, Ha]
-        simp
-      constructor <;> apply this <;> first | assumption | rw [join_commutative] <;> assumption
-    · intro ⟨ Hx, Hy ⟩
-      simp [Hx, Hy]
+theorem join_eq_bot_iff_bot : ∀ {x y : α}, x ⊔ y = ⊥ ↔ x = ⊥ ∧ y = ⊥ := by
+  intros x y
+  constructor
+  · intros H
+    have : ∀ (a b : α), a ⊔ b = ⊥ → a = ⊥ := by
+      intros a b Ha
+      have : a = a ⊓ (a ⊔ b) := by simp
+      rw [this, Ha]
+      simp
+    constructor <;> apply this <;> first | assumption | rw [join_commutative] <;> assumption
+  · intro ⟨ Hx, Hy ⟩
+    simp [Hx, Hy]
 
-  theorem meet_not_bot_left : ∀ {x y : α}, x ⊓ y ≠ ⊥ → x ≠ ⊥ := by
-    intros x y H Hc
-    apply H
-    rw [Hc, meet_commutative]
-    simp
+theorem meet_not_bot_left : ∀ {x y : α}, x ⊓ y ≠ ⊥ → x ≠ ⊥ := by
+  intros x y H Hc
+  apply H
+  rw [Hc, meet_commutative]
+  simp
 
-  theorem meet_not_bot_right : ∀ {x y : α}, x ⊓ y ≠ ⊥ → y ≠ ⊥ := by
-    intros x y H Hc
-    apply H
-    rw [Hc]
-    simp
+theorem meet_not_bot_right : ∀ {x y : α}, x ⊓ y ≠ ⊥ → y ≠ ⊥ := by
+  intros x y H Hc
+  apply H
+  rw [Hc]
+  simp
 
-  instance is_bot_dec [DecidableEq α] : DecidablePred (@is_bot α ι) := by
-    rename_i ι'
-    intros _
-    apply ι'
+instance [DecidableEq α] : DecidablePred (@IsBot α ι) := by
+  rename_i ι'
+  intros _
+  apply ι'
 
-  instance is_subset_dec [DecidableEq α] : DecidableRel (@is_subset α ι) := by
-    rename_i ι'
-    intros _ _
-    apply ι'
+instance [DecidableEq α] : DecidableRel (@IsSubset α ι) := by
+  rename_i ι'
+  intros _ _
+  apply ι'
 
-  def is_increasing : (Nat → α) → Prop :=
-    fun x => ∀ n, x n ⊑ x (n+1)
+def IsIncreasing : (Nat → α) → Prop :=
+  fun x => ∀ n, x n ⊑ x (n+1)
 
-  def is_decreasing : (Nat → α) → Prop :=
-    fun x => ∀ n, x (n+1) ⊑ x n
+def IsDecreasing : (Nat → α) → Prop :=
+  fun x => ∀ n, x (n+1) ⊑ x n
 
-  @[simp]
-  theorem join_idempotent : ∀ x : α, x ⊔ x = x := by
-    intros x
-    conv =>
-      lhs
-      arg 2
-      rw [←meet_top x]
-    apply join_absorption
+@[simp]
+theorem join_idempotent : ∀ x : α, x ⊔ x = x := by
+  intros x
+  conv =>
+    lhs
+    arg 2
+    rw [←meet_top x]
+  apply join_absorption
 
-  @[simp]
-  theorem meet_idempotent : ∀ x : α, x ⊓ x = x := by
-    intros x
-    conv =>
-      lhs
-      arg 2
-      rw [←join_bot x]
-    apply meet_absorption
+@[simp]
+theorem meet_idempotent : ∀ x : α, x ⊓ x = x := by
+  intros x
+  conv =>
+    lhs
+    arg 2
+    rw [←join_bot x]
+  apply meet_absorption
 
-  theorem refl : ∀ {x : α}, x ⊑ x := by
-    intros x
-    simp [is_subset]
+theorem refl : ∀ {x : α}, x ⊑ x := by
+  intros x
+  simp [IsSubset]
 
-  @[simp]
-  theorem meet_min_left : ∀ {x y : α}, x ⊓ y ⊑ x := by
-    intros x y
-    simp [is_subset]
-    conv =>
-      rhs
-      arg 2
-      rw [meet_commutative]
-    rw [←meet_associative]
-    simp
-
-  @[simp]
-  theorem meet_min_right : ∀ {x y : α}, x ⊓ y ⊑ y := by
-    intros x y
+@[simp]
+theorem meet_min_left : ∀ {x y : α}, x ⊓ y ⊑ x := by
+  intros x y
+  simp [IsSubset]
+  conv =>
+    rhs
+    arg 2
     rw [meet_commutative]
-    apply meet_min_left
+  rw [←meet_associative]
+  simp
+
+@[simp]
+theorem meet_min_right : ∀ {x y : α}, x ⊓ y ⊑ y := by
+  intros x y
+  rw [meet_commutative]
+  apply meet_min_left
 
 end BoundedLattice
 
@@ -178,12 +178,12 @@ export Widen (widen)
 macro l:term " ∇_" n:term:max r:term : term => ``(widen $l $r $n)
 
 namespace Widen
-  variable {α : Type} [Widen α]
+variable {α : Type} [Widen α]
 
-  @[simp]
-  def widen_seq (x : Nat → α) : Nat → α
+@[simp]
+def widenSeq (x : Nat → α) : Nat → α
   | 0 => x 0
-  | .succ n => (widen_seq x n) ∇_n (x n.succ)
+  | .succ n => (widenSeq x n) ∇_n (x n.succ)
 end Widen
 
 class WidenLawful (α : Type)
@@ -201,9 +201,9 @@ namespace Narrow
   variable {α : Type} [Narrow α]
 
   @[simp]
-  def narrow_seq (x : Nat → α) (n : Nat) : α := match n with
+  def narrowSeq (x : Nat → α) (n : Nat) : α := match n with
   | 0 => x 0
-  | .succ n => Narrow.narrow (narrow_seq x n) (x n.succ) n
+  | .succ n => Narrow.narrow (narrowSeq x n) (x n.succ) n
 end Narrow
 
 class NarrowLawful (α : Type)
